Start refactoring case study

io/DM.IIO.fst
@@ -139,22 +139,3 @@ sub_effect DM.IO.IOwp ~> IIOwp = lift_iowp_iiowp
 let get_trace () : IIOwp trace
   (fun p h -> forall lt. lt == [] ==>  p lt h) =
   IIOwp?.reflect (iio_call GetTrace ())
-
-let iio_post
-  (#a:Type)
-  (pi : monitorable_prop)
-  (h:trace)
-  (result:a)
-  (local_trace:trace) :
-  Tot bool =
-  enforced_locally pi h local_trace
-
-effect IIOpi
-  (a:Type)
-  (pi : monitorable_prop)
-  (pre : trace -> Type0)
-  (post : trace -> a -> trace -> Type0) =
-  IIOwp a
-    (fun p h ->
-      pre h /\
-      (forall r lt. (iio_post pi h r lt /\ post h r lt) ==> p lt r))
