io/TC.Monitorable.fst
@@ -5,6 +5,26 @@ open FStar.Tactics.Typeclasses
 
 open IO.Sig 
 
+type action_type = (cmd : io_cmds) & (io_sig.args cmd)
+type monitorable_prop = (history:trace) -> (action:action_type) -> Tot bool
+
+let convert_event_to_action (e:event) : action_type =
+  match e with
+  | EOpenfile arg _ -> (| Openfile, arg |)
+  | ERead arg _ -> (| Read, arg |)
+  | EClose arg _ -> (| Close, arg |)
+
+let rec enforced_locally
+  (check : monitorable_prop)
+  (h l: trace) :
+  Tot bool (decreases l) =
+  match l with
+  | [] -> true
+  | hd  ::  t ->
+    let action = convert_event_to_action hd in
+    if check h action then enforced_locally (check) (hd::h) t
+    else false
+
 class monitorable_post (#t1:Type) (#t2:Type) 
   (pre : t1 -> trace -> Type0)
   (post : t1 -> trace -> t2 -> trace -> Type0)
