io/case-studies/IO.Sig.fst
@@ -3,26 +3,62 @@ module IO.Sig
 open FStar.List.Tot.Base
 
 open Common
+include Types
 include Free
 include Hist
 
-type cmds = | Openfile | Read | Close | GetTrace
+type cmds =
+  (* files *)
+  | Openfile 
+  (* file descriptors *)
+  | Read 
+  | Write
+  | Close
+  (* sockets *)
+  | Socket
+  | Setsockopt
+  | Bind
+  | SetNonblock
+  | Listen
+  | Accept
+  | Select
+  (* instrumentation *)
+  | GetTrace
 
 (** the io free monad does not contain the GetTrace step **)
-let _io_cmds x : bool = x = Openfile || x = Read || x = Close
-type io_cmds : Type = x:cmds{_io_cmds x}
+let _io_cmds x : bool = 
+  x = Openfile || x = Read || x = Write || x = Close || 
+  x = Socket || x = Setsockopt || x = Bind || x = SetNonblock ||
+  x = Listen || x = Accept || x = Select
+type io_cmds = x:cmds{_io_cmds x}
 
 unfold let io_args (cmd:io_cmds) : Type =
   match cmd with
-  | Openfile -> string
-  | Read -> file_descr
+  | Openfile -> string * (list open_flag) * zfile_perm
+  | Read -> file_descr * UInt8.t
+  | Write -> file_descr * Bytes.bytes
   | Close -> file_descr
+  | Socket -> unit
+  | Setsockopt -> file_descr * socket_bool_option * bool
+  | Bind -> file_descr * string * UInt8.t
+  | SetNonblock -> file_descr
+  | Listen -> file_descr * UInt8.t
+  | Accept -> file_descr
+  | Select -> lfds * lfds * lfds * UInt8.t
 
 unfold let io_res (cmd:io_cmds) : Type =
   match cmd with
   | Openfile -> file_descr
-  | Read -> string
+  | Read -> Bytes.bytes * UInt8.t
+  | Write -> unit
   | Close -> unit
+  | Socket -> file_descr
+  | Setsockopt -> unit
+  | Bind -> unit
+  | SetNonblock -> unit
+  | Listen -> unit
+  | Accept -> file_descr
+  | Select -> lfds * lfds * lfds 
 
 let io_resm (cmd:io_cmds) = either (io_res cmd) exn
 
@@ -36,7 +72,15 @@ noeq
 type event =
   | EOpenfile : a:io_sig.args Openfile -> (r:io_sig.res Openfile a) -> event
   | ERead     : a:io_sig.args Read     -> (r:io_sig.res Read a)     -> event
+  | EWrite     : a:io_sig.args Write     -> (r:io_sig.res Write a)     -> event
   | EClose    : a:io_sig.args Close    -> (r:io_sig.res Close a)    -> event
+  | ESocket     : a:io_sig.args Socket     -> (r:io_sig.res Socket a)     -> event
+  | ESetsockopt     : a:io_sig.args Setsockopt     -> (r:io_sig.res Setsockopt a)     -> event
+  | EBind     : a:io_sig.args Bind     -> (r:io_sig.res Bind a)     -> event
+  | ESetNonblock     : a:io_sig.args SetNonblock     -> (r:io_sig.res SetNonblock a)     -> event
+  | EListen     : a:io_sig.args Listen     -> (r:io_sig.res Listen a)     -> event
+  | EAccept     : a:io_sig.args Accept     -> (r:io_sig.res Accept a)     -> event
+  | ESelect     : a:io_sig.args Select     -> (r:io_sig.res Select a)     -> event
 
 let hist = Hist.hist #event
 
@@ -95,7 +139,15 @@ let convert_call_to_event
   match cmd with
   | Openfile -> EOpenfile arg r
   | Read     -> ERead arg r
-  | Close    -> EClose arg r
+  | Write -> EWrite arg r
+  | Close -> EClose arg r
+  | Socket -> ESocket arg r
+  | Setsockopt -> ESetsockopt arg r
+  | Bind -> EBind arg r
+  | SetNonblock -> ESetNonblock arg r
+  | Listen -> EListen arg r
+  | Accept -> EAccept arg r
+  | Select -> ESelect arg r
 
 // OTHER TYPES & UTILS
 unfold
@@ -106,7 +158,15 @@ let destruct_event (e:event) : ( cmd:io_cmds & (arg:io_sig.args cmd) & io_sig.re
   match e with
   | EOpenfile arg res -> (| Openfile, arg, res |)
   | ERead arg res -> (| Read, arg, res |)
+  | EWrite arg res -> (| Write, arg, res |)
   | EClose arg res -> (| Close, arg, res |)
+  | ESocket arg res -> (| Socket, arg, res |)
+  | ESetsockopt arg res -> (| Setsockopt, arg, res |)
+  | EBind arg res -> (| Bind, arg, res |)
+  | ESetNonblock arg res -> (| SetNonblock, arg, res |)
+  | EListen arg res -> (| Listen, arg, res |)
+  | EAccept arg res -> (| Accept, arg, res |)
+  | ESelect arg res -> (| Select, arg, res |)
 
 let rec is_open (fd:file_descr) (h:trace) : bool =
   match h with
@@ -122,9 +182,7 @@ let rec is_open (fd:file_descr) (h:trace) : bool =
 
 unfold let io_pre (cmd:io_cmds) (arg:io_args cmd) (h:trace) : Type0 =
   match cmd with
-  | Openfile -> True
-  | Read -> is_open arg h
-  | Close -> is_open arg h
+  | _ -> True
 
 unfold let iio_wps (cmd:iio_cmds) (arg:iio_sig.args cmd) : hist (iio_sig.res cmd arg) = fun p h ->
   match cmd with
