io/model/Model.fst
@@ -4,7 +4,7 @@ open FStar.List.Tot
 open FStar.Calc
 open FStar.Tactics
 
-open Free.IO
+open IO.Sig
 open Common
 open ExtraTactics
 open TC.Monitorable
